completed until task 5

term-project.v
@@ -215,68 +215,62 @@ Definition specification_of_interpret (interpret : source_program -> expressible
     forall ae : arithmetic_expression,
       interpret (Source_program ae) = evaluate ae.
 
-
-(* Task 1: 
+(* Task 1:
    a. time permitting, prove that each of the definitions above specifies at most one function;
    b. implement these two functions; and
    c. verify that each of your functions satisfies its specification.
 *)
 
-Fixpoint evaluate_cps (ae : arithmetic_expression)
-         (k : nat -> expressible_value) : expressible_value :=
+Fixpoint evaluate_cps (ae : arithmetic_expression) (k : nat -> expressible_value) : expressible_value :=
   match ae with
   | Literal n =>
     k n
   | Plus ae1 ae2 =>
     evaluate_cps ae1 (fun n1 =>
-                        evaluate_cps ae2 (fun n2 => k (n1 + n2)))
+                        evaluate_cps ae2 (fun n2 =>
+                                            k (n1 + n2)))
   | Minus ae1 ae2 =>
-     evaluate_cps ae1 (fun n1 =>
-                         evaluate_cps ae2
-                                      (fun n2 =>
-                                         match n1 <? n2 with
-                                         | true =>
-                                           Expressible_msg
-                                             (String.append "numerical underflow: -"
-                                                            (string_of_nat (n2 - n1)))
-                                         | false =>
-                                           k (n1 - n2)
-                                         end))
+    evaluate_cps ae1 (fun n1 =>
+                        evaluate_cps ae2 (fun n2 =>
+                                            match n1 <? n2 with
+                                            | true =>
+                                              Expressible_msg
+                                                (String.append "numerical underflow: -" (string_of_nat (n2 - n1)))
+                                            | false =>
+                                              k (n1 - n2)
+                                            end))
   end.
 
-Definition evaluate (ae : arithmetic_expression) :=
-  evaluate_cps ae (fun n => Expressible_nat n).
-
-Compute (evaluate (Plus (Plus (Literal 1) (Literal 2)) (Literal 2 ))).
-Compute (evaluate (Minus (Literal 1) (Literal 2))).
-
-
 Lemma fold_unfold_evaluate_cps_Literal :
-  forall (n : nat) (k : nat -> expressible_value),
-    evaluate_cps (Literal n) k = k n.
+  forall (n : nat)
+         (k : nat -> expressible_value),
+    evaluate_cps (Literal n) k =
+    k n.
 Proof.
   fold_unfold_tactic evaluate_cps.
 Qed.
 
 Lemma fold_unfold_evaluate_cps_Plus :
-  forall (ae1 ae2 : arithmetic_expression) (k : nat -> expressible_value),
+  forall (ae1 ae2 : arithmetic_expression)
+         (k : nat -> expressible_value),
     evaluate_cps (Plus ae1 ae2) k =
     evaluate_cps ae1 (fun n1 =>
-                        evaluate_cps ae2 (fun n2 => k (n1 + n2))).
+                        evaluate_cps ae2 (fun n2 =>
+                                            k (n1 + n2))).
 Proof.
   fold_unfold_tactic evaluate_cps.
 Qed.
 
 Lemma fold_unfold_evaluate_cps_Minus :
-  forall (ae1 ae2 : arithmetic_expression) (k : nat -> expressible_value),
+  forall (ae1 ae2 : arithmetic_expression)
+         (k : nat -> expressible_value),
     evaluate_cps (Minus ae1 ae2) k =
     evaluate_cps ae1 (fun n1 =>
                         evaluate_cps ae2 (fun n2 =>
                                             match n1 <? n2 with
                                             | true =>
                                               Expressible_msg
-                                                (String.append "numerical underflow: -"
-                                                               (string_of_nat (n2 - n1)))
+                                                (String.append "numerical underflow: -" (string_of_nat (n2 - n1)))
                                             | false =>
                                               k (n1 - n2)
                                             end)).
@@ -301,147 +295,333 @@ Lemma about_evaluate_cps :
             evaluate_cps ae k = Expressible_msg s).
 Proof.
   intros evaluate S_evaluate ae.
-  induction ae as [n
-                  | ae1 [[n1  [IHae1 IHae1_cps]] | [s1 [IHae1 IHae1_cps]]]
-                        ae2 [[n2  [IHae2 IHae2_cps]] | [s2  [IHae2 IHae2_cps]]]
-                  | ae1 [[n1  [IHae1 IHae1_cps]] | [s1 [IHae1 IHae1_cps]]]
-                        ae2 [[n2  [IHae2 IHae2_cps]] | [s2  [IHae2 IHae2_cps]]]];
-    unfold specification_of_evaluate in S_evaluate.
-  (* ae is Literal *)
-  + left.
+  induction ae as [n |
+                   ae1 [[n1 [IHae1 IHae1_cps]] | [s1 [IHae1 IHae1_cps]]] ae2 [[n2 [IHae2 IHae2_cps]] | [s2 [IHae2 IHae2_cps]]] |
+                   ae1 [[n1 [IHae1 IHae1_cps]] | [s1 [IHae1 IHae1_cps]]] ae2 [[n2 [IHae2 IHae2_cps]] | [s2 [IHae2 IHae2_cps]]]].
+  - unfold specification_of_evaluate in S_evaluate.
     destruct S_evaluate as [S_Literal _].
+    left.
     exists n.
     split.
-    ++ exact (S_Literal n).
-    ++ intro k.
-       rewrite -> fold_unfold_evaluate_cps_Literal.
-       reflexivity.
-    (* ae is Plus *)
-  + left.
-    destruct S_evaluate as [_ [[_ [_ S_Plus_n1n2]] _]].
-    Check (S_Plus_n1n2 ae1 ae2 n1 n2 IHae1 IHae2).
+    + exact (S_Literal n).
+    + intro k.
+      rewrite -> fold_unfold_evaluate_cps_Literal.
+      reflexivity.
+  - unfold specification_of_evaluate in S_evaluate.
+    destruct S_evaluate as [_ [[_ [_ S_Plus_n1_n2]] _]].
+    Check (S_Plus_n1_n2
+             ae1
+             ae2
+             n1
+             n2
+             IHae1
+             IHae2).
+    left.
     exists (n1 + n2).
     split.
-    ++ exact (S_Plus_n1n2 ae1 ae2 n1 n2 IHae1 IHae2).
-    ++ intro k.
-       rewrite -> fold_unfold_evaluate_cps_Plus.
-       Check (IHae1_cps (fun n0 : nat =>
-                           evaluate_cps ae2 (fun n3 : nat => k (n0 + n3)))).
-       rewrite -> (IHae1_cps (fun n0 : nat =>
-                                evaluate_cps ae2 (fun n3 : nat => k (n0 + n3)))).
-       rewrite -> (IHae2_cps (fun n0 : nat => k (n1 + n0))).
-       reflexivity.
-  + right.
+    + exact (S_Plus_n1_n2
+             ae1
+             ae2
+             n1
+             n2
+             IHae1
+             IHae2).
+    + intro k.
+      rewrite -> fold_unfold_evaluate_cps_Plus.
+      Check (IHae1_cps (fun n0 : nat => evaluate_cps ae2 (fun n3 : nat => k (n0 + n3)))).
+      rewrite -> (IHae1_cps (fun n0 : nat => evaluate_cps ae2 (fun n3 : nat => k (n0 + n3)))).
+      rewrite -> (IHae2_cps (fun n3 : nat => k (n1 + n3))).
+      reflexivity.
+  - right.
+    unfold specification_of_evaluate in S_evaluate.
     destruct S_evaluate as [_ [[_ [S_Plus_n1_s2 _]] _]].
-    Check (S_Plus_n1_s2 ae1 ae2 n1 s2 IHae1 IHae2).
+    Check (S_Plus_n1_s2
+             ae1
+             ae2
+             n1
+             s2
+             IHae1
+             IHae2).
     exists s2.
     split.
-    ++ exact (S_Plus_n1_s2 ae1 ae2 n1 s2 IHae1 IHae2).
-    ++ intro k.
-       rewrite -> fold_unfold_evaluate_cps_Plus.
-       rewrite -> (IHae1_cps (fun n0 : nat =>
-                               evaluate_cps ae2 (fun n2 : nat => k (n0 + n2)))).
-       rewrite -> (IHae2_cps (fun n2 : nat => k (n1 + n2))).
-       reflexivity.
-  + right.
+    + exact (S_Plus_n1_s2
+             ae1
+             ae2
+             n1
+             s2
+             IHae1
+             IHae2).
+    + intro k.
+      rewrite -> fold_unfold_evaluate_cps_Plus.
+      rewrite -> (IHae1_cps (fun n0 : nat => evaluate_cps ae2 (fun n2 : nat => k (n0 + n2)))).
+      rewrite -> (IHae2_cps (fun n2 : nat => k (n1 + n2))).
+      reflexivity.
+  - right.
+    unfold specification_of_evaluate in S_evaluate.
     destruct S_evaluate as [_ [[S_Plus_s1_n2 [_ _]] _]].
+    Check (S_Plus_s1_n2
+             ae1
+             ae2
+             s1
+             IHae1).
     exists s1.
     split.
-    ++ exact (S_Plus_s1_n2 ae1 ae2 s1 IHae1).
-    ++ intro k.
-       rewrite -> fold_unfold_evaluate_cps_Plus.
-       rewrite -> IHae1_cps.
-       reflexivity.
-  + right.
-    exists s1.
+    + exact (S_Plus_s1_n2
+             ae1
+             ae2
+             s1
+             IHae1).
+    + intro k.
+      rewrite -> fold_unfold_evaluate_cps_Plus.
+      rewrite -> (IHae1_cps (fun n1 : nat => evaluate_cps ae2 (fun n0 : nat => k (n1 + n0)))).
+      reflexivity.
+  - right.
+    unfold specification_of_evaluate in S_evaluate.
     destruct S_evaluate as [_ [[S_Plus_s1_n2 [_ _]] _]].
+    exists s1.
+    Check (S_Plus_s1_n2 ae1 ae2 s1 IHae1).
     split.
-    ++ exact (S_Plus_s1_n2 ae1 ae2 s1 IHae1).
-    ++ intro k.
-       rewrite -> fold_unfold_evaluate_cps_Plus.
-       rewrite -> (IHae1_cps
-                     (fun n1 : nat =>
-                        evaluate_cps ae2 (fun n2 : nat => k (n1 + n2)))).
-       reflexivity.
-   (* ae is Minus *)
-  + case (n1 <? n2) eqn:H_n1_n2.
-    ++ right.
-       destruct S_evaluate as [_ [_ [_ [_ [S_Minus_n1_n2_msg _]]]]].
-       Check (S_Minus_n1_n2_msg ae1 ae2 n1 n2 IHae1 IHae2 H_n1_n2).
-       exists (String.append
-                 "numerical underflow: -" (string_of_nat (n2 - n1))).
-       split.
-       +++ exact (S_Minus_n1_n2_msg ae1 ae2 n1 n2 IHae1 IHae2 H_n1_n2).
-       +++ intro k.
-           rewrite -> fold_unfold_evaluate_cps_Minus.
-           rewrite -> IHae1_cps.
-           rewrite -> IHae2_cps.
-           rewrite -> H_n1_n2.
-           reflexivity.
-    ++ left.
-       destruct S_evaluate as [_ [_ [_ [_ [_ S_Minus_n1_n2_nat]]]]].
-       Check (S_Minus_n1_n2_nat ae1 ae2 n1 n2 IHae1 IHae2 H_n1_n2).
-       exists (n1 - n2).
-       split.
-       +++ exact (S_Minus_n1_n2_nat ae1 ae2 n1 n2 IHae1 IHae2 H_n1_n2).
-       +++ intro k.
-           rewrite -> fold_unfold_evaluate_cps_Minus.
-           rewrite -> IHae1_cps.
-           rewrite -> IHae2_cps.
-           rewrite -> H_n1_n2.
-           reflexivity.
-  + right.
+    + exact (S_Plus_s1_n2 ae1 ae2 s1 IHae1).
+    + intro k.
+      rewrite -> fold_unfold_evaluate_cps_Plus.
+      rewrite -> (IHae1_cps (fun n1 : nat => evaluate_cps ae2 (fun n2 : nat => k (n1 + n2)))).
+      reflexivity.
+  - case (n1 <? n2) eqn:H_n1_n2.
+    + right.
+      unfold specification_of_evaluate in S_evaluate.
+      destruct S_evaluate as [_ [_ [_ [_ [S_Minus_n1_n2_msg _]]]]].
+      Check (S_Minus_n1_n2_msg ae1 ae2 n1 n2 IHae1 IHae2 H_n1_n2).
+      exists (String.append "numerical underflow: -" (string_of_nat (n2 - n1))).
+      split.
+      * exact (S_Minus_n1_n2_msg ae1 ae2 n1 n2 IHae1 IHae2 H_n1_n2).
+      * intro k.
+        rewrite -> fold_unfold_evaluate_cps_Minus.
+        rewrite -> (IHae1_cps (fun n0 : nat =>
+                                 evaluate_cps ae2
+                                              (fun n3 : nat =>
+                                                 if n0 <? n3
+                                                 then
+                                                   Expressible_msg
+                                                     ("numerical underflow: -" ++ string_of_nat (n3 - n0))
+                                                 else k (n0 - n3)))).
+        rewrite -> (IHae2_cps (fun n3 : nat =>
+                                 if n1 <? n3
+                                 then
+                                   Expressible_msg ("numerical underflow: -" ++ string_of_nat (n3 - n1))
+                                 else k (n1 - n3))).
+        rewrite -> H_n1_n2.
+        reflexivity.
+    + left.
+      unfold specification_of_evaluate in S_evaluate.
+      destruct S_evaluate as [_ [_ [_ [_ [_ S_Minus_n1_n2_nat]]]]].
+      Check (S_Minus_n1_n2_nat ae1 ae2 n1 n2 IHae1 IHae2 H_n1_n2).
+      exists (n1 - n2).
+      split.
+      * exact (S_Minus_n1_n2_nat ae1 ae2 n1 n2 IHae1 IHae2 H_n1_n2).
+      * intro k.
+        rewrite -> fold_unfold_evaluate_cps_Minus.
+        rewrite -> (IHae1_cps (fun n0 : nat =>
+                                 evaluate_cps ae2
+                                              (fun n3 : nat =>
+                                                 if n0 <? n3
+                                                 then
+                                                   Expressible_msg
+                                                     ("numerical underflow: -" ++ string_of_nat (n3 - n0))
+                                                 else k (n0 - n3)))).
+        rewrite -> (IHae2_cps (fun n3 : nat =>
+                                 if n1 <? n3
+                                 then
+                                   Expressible_msg ("numerical underflow: -" ++ string_of_nat (n3 - n1))
+                                 else k (n1 - n3))).
+        rewrite -> H_n1_n2.
+        reflexivity.
+  - right.
+    unfold specification_of_evaluate in S_evaluate.
     destruct S_evaluate as [_ [_ [_ [S_Minus_n1_s2 _]]]].
-    Check (S_Minus_n1_s2 ae1 ae2 n1 s2 IHae1 IHae2).
+    Check (S_Minus_n1_s2
+             ae1
+             ae2
+             n1
+             s2
+             IHae1
+             IHae2).
     exists s2.
     split.
-    ++ exact (S_Minus_n1_s2 ae1 ae2 n1 s2 IHae1 IHae2).
-    ++ intro k.
-       rewrite -> fold_unfold_evaluate_cps_Minus.
-       rewrite -> IHae1_cps.
-       rewrite -> IHae2_cps.
-       reflexivity.
-  + right.
-    destruct S_evaluate as [_ [_ [S_Minus_s1_n2 _]]].
+    + exact (S_Minus_n1_s2
+             ae1
+             ae2
+             n1
+             s2
+             IHae1
+             IHae2).
+    + intro k.
+      rewrite -> fold_unfold_evaluate_cps_Minus.
+      rewrite -> (IHae1_cps (fun n0 : nat =>
+                               evaluate_cps ae2
+                                            (fun n2 : nat =>
+                                               if n0 <? n2
+                                               then
+                                                 Expressible_msg
+                                                   ("numerical underflow: -" ++ string_of_nat (n2 - n0))
+                                               else k (n0 - n2)))).
+      rewrite -> (IHae2_cps (fun n2 : nat =>
+                               if n1 <? n2
+                               then
+                                 Expressible_msg ("numerical underflow: -" ++ string_of_nat (n2 - n1))
+                               else k (n1 - n2))).
+      reflexivity.
+  - unfold specification_of_evaluate in S_evaluate.
+    destruct S_evaluate as [_ [_ [S_Minus_s1_n2 [_ _]]]].
     Check (S_Minus_s1_n2 ae1 ae2 s1 IHae1).
+    right.
     exists s1.
     split.
-    ++ exact (S_Minus_s1_n2 ae1 ae2 s1 IHae1).
-    ++ intro k.
-       rewrite -> fold_unfold_evaluate_cps_Minus.
-       rewrite -> IHae1_cps.
-       reflexivity.
-  + right.
-    destruct S_evaluate as [_ [_ [S_Minus_s1_n2 _]]].
-    Check (S_Minus_s1_n2 ae1 ae2 s1 IHae1).
+    + exact (S_Minus_s1_n2 ae1 ae2 s1 IHae1).
+    + intro k.
+      rewrite -> fold_unfold_evaluate_cps_Minus.
+      rewrite -> (IHae1_cps (fun n1 : nat =>
+                               evaluate_cps ae2
+                                            (fun n0 : nat =>
+                                               if n1 <? n0
+                                               then
+                                                 Expressible_msg
+                                                   ("numerical underflow: -" ++ string_of_nat (n0 - n1))
+                                               else k (n1 - n0)))).
+      reflexivity.
+  - right.
+    unfold specification_of_evaluate in S_evaluate.
+    destruct S_evaluate as [_ [_ [S_Minus_s1_n2 [_ _]]]].
     exists s1.
+    Check (S_Minus_s1_n2 ae1 ae2 s1 IHae1).
     split.
-    ++ exact (S_Minus_s1_n2 ae1 ae2 s1 IHae1).
-    ++ intro k.
-       rewrite -> fold_unfold_evaluate_cps_Minus.
-       rewrite -> IHae1_cps.
-       reflexivity.
+    + exact (S_Minus_s1_n2 ae1 ae2 s1 IHae1).
+    + intro k.
+      rewrite -> fold_unfold_evaluate_cps_Minus.
+      rewrite -> (IHae1_cps (fun n1 : nat =>
+                               evaluate_cps ae2
+                                            (fun n2 : nat =>
+                                               if n1 <? n2
+                                               then
+                                                 Expressible_msg
+                                                   ("numerical underflow: -" ++ string_of_nat (n2 - n1))
+                                               else k (n1 - n2)))).
+      reflexivity.
 Qed.
 
+Fixpoint evaluate (ae: arithmetic_expression) : expressible_value :=
+  match ae with
+  | Literal n =>
+    Expressible_nat n
+  | Plus ae1 ae2  =>
+    match evaluate ae1 with
+    | Expressible_msg s1 => Expressible_msg s1
+    | Expressible_nat n1 => match evaluate ae2 with
+                            | Expressible_msg s2 => Expressible_msg s2
+                            | Expressible_nat n2 => Expressible_nat (n1 + n2)
+                            end
+    end
+  | Minus ae1 ae2  =>
+    match evaluate ae1 with
+    | Expressible_msg s1 => Expressible_msg s1
+    | Expressible_nat n1 => match evaluate ae2 with
+                            | Expressible_msg s2 => Expressible_msg s2
+                            | Expressible_nat n2 =>
+                              if n1 <? n2
+                              then Expressible_msg
+                                     (String.append "numerical underflow: -" (string_of_nat (n2 - n1)))
+                              else Expressible_nat (n1 - n2)
+                            end
+    end
+  end.
 
-(* probably wrong way to go about it *)
+Lemma fold_unfold_evaluate_Literal :
+  forall (n : nat),
+    evaluate (Literal n) =
+    Expressible_nat n.
+Proof.
+  fold_unfold_tactic evaluate.
+Qed.
+
+Lemma fold_unfold_evaluate_Plus :
+  forall (ae1 ae2 : arithmetic_expression),
+    evaluate (Plus ae1 ae2) =
+    match evaluate ae1 with
+    | Expressible_msg s1 => Expressible_msg s1
+    | Expressible_nat n1 => match evaluate ae2 with
+                            | Expressible_msg s2 => Expressible_msg s2
+                            | Expressible_nat n2 => Expressible_nat (n1 + n2)
+                            end
+    end.
+Proof.
+  fold_unfold_tactic evaluate.
+Qed.
+
+Lemma fold_unfold_evaluate_Minus :
+  forall (ae1 ae2 : arithmetic_expression),
+    evaluate (Minus ae1 ae2) =
+    match evaluate ae1 with
+    | Expressible_msg s1 => Expressible_msg s1
+    | Expressible_nat n1 => match evaluate ae2 with
+                            | Expressible_msg s2 => Expressible_msg s2
+                            | Expressible_nat n2 =>
+                              if n1 <? n2
+                              then Expressible_msg
+                                     (String.append "numerical underflow: -" (string_of_nat (n2 - n1)))
+                              else Expressible_nat (n1 - n2)
+                            end
+    end.
+Proof.
+  fold_unfold_tactic evaluate.
+Qed.
+
 Theorem evaluate_satisfies_the_specification_of_evaluate :
   specification_of_evaluate evaluate.
 Proof.
-  unfold evaluate, specification_of_evaluate.
-  split.
-  + intro n.
-    rewrite -> fold_unfold_evaluate_cps_Literal.
+  unfold specification_of_evaluate.
+  repeat split; intros ae1 ae2; (rewrite -> (fold_unfold_evaluate_Literal) || rewrite -> (fold_unfold_evaluate_Plus) || rewrite -> (fold_unfold_evaluate_Minus)).
+  - intros s1 H_evaluate_ae1.
+    rewrite -> H_evaluate_ae1.
     reflexivity.
-  + split; split.
-    ++ intros ae1 ae2 s1 IHae.
-       rewrite -> fold_unfold_evaluate_cps_Plus.
-       Admitted.
-           
-          
+  - intros n1 n2 H_evaluate_ae1 H_evaluate_ae2.
+    rewrite -> H_evaluate_ae1.
+    rewrite -> H_evaluate_ae2.
+    reflexivity.
+  - intros n1 n2 H_evaluate_ae1 H_evaluate_ae2.
+    rewrite -> H_evaluate_ae1.
+    rewrite -> H_evaluate_ae2.
+    reflexivity.
+  - intros s1 H_evaluate_ae1.
+    rewrite -> H_evaluate_ae1.
+    reflexivity.
+  - intros n1 n2 H_evaluate_ae1 H_evaluate_ae2.
+    rewrite -> H_evaluate_ae1.
+    rewrite -> H_evaluate_ae2.
+    reflexivity.
+  - intros n1 n2 H_evaluate_ae1 H_evaluate_ae2 H_lesser_than.
+    rewrite -> H_evaluate_ae1.
+    rewrite -> H_evaluate_ae2.
+    rewrite -> H_lesser_than.
+    reflexivity.
+  - intros n1 n2 H_evaluate_ae1 H_evaluate_ae2 H_lesser_than.
+    rewrite -> H_evaluate_ae1.
+    rewrite -> H_evaluate_ae2.
+    rewrite -> H_lesser_than.
+    reflexivity.
+
+    Restart.
+    unfold specification_of_evaluate.
+    repeat split;
+      intros ae1 ae2;
+      (rewrite -> (fold_unfold_evaluate_Literal) ||
+       rewrite -> (fold_unfold_evaluate_Plus) ||
+       rewrite -> (fold_unfold_evaluate_Minus));
+      ((intros s1 H_evaluate_ae1; rewrite -> H_evaluate_ae1; reflexivity) ||
+       (intros n1 n2 H_evaluate_ae1 H_evaluate_ae2; rewrite -> H_evaluate_ae1; rewrite -> H_evaluate_ae2;  reflexivity) ||
+       (intros n1 n2 H_evaluate_ae1 H_evaluate_ae2 H_lesser_than; rewrite -> H_evaluate_ae1; rewrite -> H_evaluate_ae2; rewrite -> H_lesser_than; reflexivity)).
+    Qed.
 
 Definition interpret (sp : source_program) : expressible_value :=
-    match sp with
+  match sp with
   | Source_program ae =>
     evaluate_cps ae (fun (n : nat) => Expressible_nat n)
   end.
@@ -451,39 +631,25 @@ Theorem interpret_satisfies_the_specification_of_interpret :
 Proof.
   unfold specification_of_interpret.
   intros evaluate S_evaluate ae.
-  Check (about_evaluate_cps evaluate S_evaluate ae).
-  destruct (about_evaluate_cps evaluate S_evaluate ae)
-    as [[n [H_eval H_eval_cps]] | [s [H_eval H_eval_cps]]];
-    unfold interpret;
-    rewrite (H_eval_cps (fun n => Expressible_nat n));
+  Check (about_evaluate_cps
+           evaluate
+           S_evaluate
+           ae).
+  destruct (about_evaluate_cps
+              evaluate
+              S_evaluate
+              ae) as [[n [H_eval H_eval_cps]] | [s [H_eval H_eval_cps]]].
+  - unfold interpret.
+    Check (H_eval_cps (fun n => Expressible_nat n)).
+    rewrite -> (H_eval_cps (fun n => Expressible_nat n)).
+    Check (eq_sym H_eval).
+    exact (eq_sym H_eval).
+  - unfold interpret.
+    Check (H_eval_cps (fun n => Expressible_nat n)).
+    rewrite -> (H_eval_cps (fun n => Expressible_nat n)).
     exact (eq_sym H_eval).
 Qed.
 
-
-(*
-Theorem there_exists_at_most_one_evaluate_function :
-  forall (ev1 ev2 : arithmetic_expression -> expressible_value),
-    specification_of_evaluate ev1 ->
-    specification_of_evaluate ev2 ->
-    forall (ae : arithmetic_expression),
-      ev1 ae = ev2 ae.
-Proof.
-  intros ev1 ev2 ev1_spec ev2_spec ae.
-  case ae.
-  + intro n.
-    destruct ev1_spec as [ev1_spec_literal _].
-    destruct ev2_spec as [ev2_spec_literal _].
-    rewrite -> ev2_spec_literal.
-    exact (ev1_spec_literal n).
-  + intros ae1 ae2.
-    destruct ev1_spec.
-    
-  destruct ev1_spec.
-
-Started but realized it was the least important on the list 
-*)
-
-  
 (* ********** *)
 
 (* Byte-code instructions: *)
@@ -537,22 +703,85 @@ Definition specification_of_decode_execute (decode_execute : byte_code_instructi
        n1 <? n2 = false ->
        decode_execute SUB (n2 :: n1 :: ds) = OK ((n1 - n2) :: ds))).
 
-
 (* Task 2:
    a. time permitting, prove that the definition above specifies at most one function;
    b. implement this function; and
    c. verify that your function satisfies the specification.
 *)
 
-(*
+Theorem there_is_at_most_one_decode_execute :
+  forall (decode_execute_1 decode_execute_2 : byte_code_instruction -> data_stack -> result_of_decoding_and_execution),
+    specification_of_decode_execute decode_execute_1 ->
+    specification_of_decode_execute decode_execute_2 ->
+    forall (bcis : byte_code_instruction)
+           (ds : data_stack),
+      decode_execute_1 bcis ds = decode_execute_2 bcis ds.
+Proof.
+  intros decode_execute_1 decode_execute_2 S_decode_execute_1 S_decode_execute_2 bcis ds.
+  destruct bcis.
+  - unfold specification_of_decode_execute in S_decode_execute_1.
+    destruct S_decode_execute_1 as [S_PUSH_1 _].
+    unfold specification_of_decode_execute in S_decode_execute_2.
+    destruct S_decode_execute_2 as [S_PUSH_2 _].
+    rewrite -> (S_PUSH_2 n ds).
+    exact (S_PUSH_1 n ds).
+  - unfold specification_of_decode_execute in S_decode_execute_1.
+    destruct S_decode_execute_1 as [ _ [[S_ADD_nil_1 [S_ADD_cons_1 S_ADD_cons_cons_1]] _]].
+    destruct S_decode_execute_2 as [ _ [[S_ADD_nil_2 [S_ADD_cons_2 S_ADD_cons_cons_2]] _]].
+    destruct ds as [ | n1].
+    -- rewrite -> S_ADD_nil_2.
+       exact (S_ADD_nil_1).
+    -- destruct ds as [ | n2].
+       --- rewrite -> (S_ADD_cons_2 n1).
+           exact (S_ADD_cons_1 n1).
+       --- rewrite -> (S_ADD_cons_cons_2 n2 n1 ds).
+           exact (S_ADD_cons_cons_1 n2 n1 ds).
+ - unfold specification_of_decode_execute in S_decode_execute_1.
+    destruct S_decode_execute_1 as [ _ [_ [S_SUB_nil_1 [S_SUB_cons_1 [S_SUB_cons_cons_lesser_than_1 S_SUB_cons_cons_not_lesser_than_1]]]]].
+    destruct S_decode_execute_2 as [ _ [_ [S_SUB_nil_2 [S_SUB_cons_2 [S_SUB_cons_cons_lesser_than_2 S_SUB_cons_cons_not_lesser_than_2]]]]].
+    destruct ds as [ | n1].
+    -- rewrite -> S_SUB_nil_2.
+       exact (S_SUB_nil_1).
+    -- destruct ds as [ | n2].
+       --- rewrite -> (S_SUB_cons_2 n1).
+           exact (S_SUB_cons_1 n1).
+       --- case (n2 <? n1) eqn:H_n2_n1.
+           ---- rewrite -> (S_SUB_cons_cons_lesser_than_2 n2 n1 ds H_n2_n1).
+                 exact (S_SUB_cons_cons_lesser_than_1 n2 n1 ds H_n2_n1).
+           ---- rewrite -> (S_SUB_cons_cons_not_lesser_than_2 n2 n1 ds H_n2_n1).
+                 exact (S_SUB_cons_cons_not_lesser_than_1 n2 n1 ds H_n2_n1).
+Qed.
+
 Definition decode_execute (bcis : byte_code_instruction) (ds : data_stack) : result_of_decoding_and_execution :=
-  ...
+  match bcis with
+  | PUSH n =>
+    OK (n :: ds)
+  | ADD =>
+    match ds with
+    | nil => KO "ADD: stack underflow"
+    | (n2 :: nil) => KO "ADD: stack underflow"
+    | (n2 :: n1 :: ds) => OK ((n1 + n2) :: ds)
+    end
+  | SUB => match ds with
+           | nil => KO "SUB: stack underflow"
+           | (n2 :: nil) => KO "SUB: stack underflow"
+           | (n2 :: n1 :: ds) => if n1 <? n2
+                                 then KO (String.append "numerical underflow: -" (string_of_nat (n2 - n1)))
+                                 else OK ((n1 - n2) :: ds)
+           end
+  end.
 
 Theorem decode_execute_satisfies_the_specification_of_decode_execute :
   specification_of_decode_execute decode_execute.
 Proof.
-Abort.
-*)
+  unfold specification_of_decode_execute.
+  repeat split; (* since there are 7 conjunctions, I thought this would result in 8 subgoals
+                   but it only gives two... *)
+  intros n1 n2 ds H_lesser_than;
+  unfold decode_execute;
+  rewrite -> H_lesser_than;
+  reflexivity.
+Qed.
 
 (* ********** *)
 
@@ -585,6 +814,101 @@ Definition specification_of_fetch_decode_execute_loop (fetch_decode_execute_loop
    c. verify that your function satisfies the specification.
 *)
 
+Fixpoint fetch_decode_execute_loop (bcis : list byte_code_instruction) (ds : data_stack) : result_of_decoding_and_execution :=
+    match bcis with
+      | nil => OK ds
+      | bci :: bcis' => match decode_execute bci ds with
+                          | OK ds' => fetch_decode_execute_loop bcis' ds'
+                          | KO s => KO s
+                        end
+    end.
+
+Lemma fold_unfold_fetch_decode_execute_loop_nil :
+  forall (ds : data_stack),
+    fetch_decode_execute_loop nil ds = OK ds.
+Proof.
+  fold_unfold_tactic fetch_decode_execute_loop.
+Qed.
+
+Lemma fold_unfold_fetch_decode_execute_loop_cons :
+  forall (bci : byte_code_instruction)
+         (bcis' : list byte_code_instruction)
+         (ds : data_stack),
+    fetch_decode_execute_loop (bci :: bcis') ds = match decode_execute bci ds with
+                                                  | OK ds' => fetch_decode_execute_loop bcis' ds'
+                                                  | KO s => KO s
+                                                  end.
+Proof.
+  fold_unfold_tactic fetch_decode_execute_loop.
+Qed.
+
+Theorem there_is_at_most_one_fetch_decode_execute_loop :
+  forall (fetch_decode_execute_loop_1 fetch_decode_execute_loop_2 :list byte_code_instruction -> data_stack -> result_of_decoding_and_execution),
+    specification_of_fetch_decode_execute_loop fetch_decode_execute_loop_1 ->
+    specification_of_fetch_decode_execute_loop fetch_decode_execute_loop_2 ->
+    forall (bcis : list  byte_code_instruction)
+           (ds : data_stack),
+      fetch_decode_execute_loop_1 bcis ds = fetch_decode_execute_loop_2 bcis ds.
+Proof.
+  intros fetch_decode_execute_loop_1 fetch_decode_execute_loop_2
+         S_fetch_decode_execute_loop_1
+         S_fetch_decode_execute_loop_2
+         bcis.
+  unfold specification_of_fetch_decode_execute_loop in S_fetch_decode_execute_loop_1.
+  assert (S_fetch_decode_execute_loop_1 :=
+            S_fetch_decode_execute_loop_1
+              decode_execute
+              decode_execute_satisfies_the_specification_of_decode_execute).
+  unfold specification_of_fetch_decode_execute_loop in S_fetch_decode_execute_loop_2.
+  assert (S_fetch_decode_execute_loop_2 :=
+            S_fetch_decode_execute_loop_2
+              decode_execute
+              decode_execute_satisfies_the_specification_of_decode_execute).
+  induction bcis as [ | bci bcis' IHbcis'].
+  - intro ds.
+    destruct S_fetch_decode_execute_loop_1 as [H_nil_1 _].
+    destruct S_fetch_decode_execute_loop_2 as [H_nil_2 _].
+    rewrite -> (H_nil_2 ds).
+    exact (H_nil_1 ds).
+  - intro ds.
+    destruct (decode_execute bci ds) as [ds' | s] eqn: H_decode_execute.
+    -- destruct S_fetch_decode_execute_loop_1 as [_ [H_decode_execute_OK_1 _]].
+       destruct S_fetch_decode_execute_loop_2 as [_ [H_decode_execute_OK_2 _]].
+       rewrite -> (H_decode_execute_OK_1 bci bcis' ds ds' H_decode_execute).
+       rewrite -> (H_decode_execute_OK_2 bci bcis' ds ds' H_decode_execute).
+       exact (IHbcis' ds').
+    -- destruct S_fetch_decode_execute_loop_1 as [_ [_ H_decode_execute_KO_1]].
+       destruct S_fetch_decode_execute_loop_2 as [_ [_ H_decode_execute_KO_2]].
+       rewrite -> (H_decode_execute_KO_2 bci bcis' ds s H_decode_execute).
+       exact (H_decode_execute_KO_1 bci bcis' ds s H_decode_execute).
+Qed.
+
+Theorem fetch_decode_execute_loop_satisfies_the_specification_of_fetch_decode_execute_loop :
+  specification_of_fetch_decode_execute_loop fetch_decode_execute_loop.
+Proof.
+  unfold specification_of_fetch_decode_execute_loop.
+  intros decode_execute0 H_decode_execute0_satisfies_the_specification_of_decode_execute.
+  repeat split; intros bci bcis' ds. 
+  - intros ds' H_decode_execute0. 
+    rewrite -> (fold_unfold_fetch_decode_execute_loop_cons bci bcis' ds).
+    rewrite -> (there_is_at_most_one_decode_execute
+                  decode_execute
+                  decode_execute0
+                  decode_execute_satisfies_the_specification_of_decode_execute
+                  H_decode_execute0_satisfies_the_specification_of_decode_execute).
+    rewrite -> (H_decode_execute0).
+    reflexivity.
+  - intros s H_decode_execute0.
+    rewrite -> (fold_unfold_fetch_decode_execute_loop_cons bci bcis' ds).
+    rewrite -> (there_is_at_most_one_decode_execute
+                  decode_execute
+                  decode_execute0
+                  decode_execute_satisfies_the_specification_of_decode_execute
+                  H_decode_execute0_satisfies_the_specification_of_decode_execute).
+    rewrite -> (H_decode_execute0).
+    reflexivity.
+Qed.
+
 (* ********** *)
 
 (* Task 4:
@@ -610,6 +934,30 @@ Lemma fold_unfold_append_cons :
     bci1 :: (bci1s ++ bci2s).
 Proof.
   fold_unfold_tactic List.app.
+Qed.
+
+Theorem execution_and_concatenation_commute :
+  forall (bcis1 bcis2 : list byte_code_instruction)
+         (ds : data_stack),
+    fetch_decode_execute_loop (bcis1 ++ bcis2) ds =
+    match fetch_decode_execute_loop bcis1 ds with
+    | OK ds_new => fetch_decode_execute_loop bcis2 ds_new
+    | KO s => KO s
+    end.
+Proof.
+  intros bcis1 bcis2.
+  induction bcis1 as [ | bci1 bcis1' IHbcis1'].
+  - intro ds.
+    rewrite -> (fold_unfold_append_nil bcis2).
+    rewrite -> (fold_unfold_fetch_decode_execute_loop_nil).
+    reflexivity.
+ - intro ds.
+   rewrite -> (fold_unfold_append_cons bci1 bcis1' bcis2).
+   rewrite -> (fold_unfold_fetch_decode_execute_loop_cons bci1 (bcis1' ++ bcis2) ds).
+   rewrite -> (fold_unfold_fetch_decode_execute_loop_cons bci1 bcis1' ds).
+   destruct (decode_execute bci1 ds) as [ds' | ds'].
+   -- exact (IHbcis1' ds').
+   -- reflexivity.
 Qed.
 
 (* ********** *)
@@ -642,6 +990,53 @@ Definition specification_of_run (run : target_program -> expressible_value) :=
    b. implement this function; and
    c. verify that your function satisfies the specification.
 *)
+
+Definition run (t : target_program) : expressible_value :=
+  match t with
+  | Target_program bcis =>
+    match fetch_decode_execute_loop bcis nil with
+    | KO s => Expressible_msg s
+    | OK ds => 
+      match ds with
+      | nil => Expressible_msg "no result on the data stack"
+      | n :: ds' => 
+        match ds' with
+        | nil => Expressible_nat n
+        | n' :: ds'' => Expressible_msg "too many results on the data stack"
+        end
+      end
+    end
+  end.
+
+Theorem run_satisfies_the_specification_of_run :
+  specification_of_run run.
+Proof.
+  unfold specification_of_run.
+  intros fetch_decode_execute_loop0 S_fetch_decode_execute_loop0.
+  repeat split;
+    intro bcis;
+    rewrite -> (there_is_at_most_one_fetch_decode_execute_loop
+                  fetch_decode_execute_loop0 
+                  fetch_decode_execute_loop
+                  S_fetch_decode_execute_loop0
+                  fetch_decode_execute_loop_satisfies_the_specification_of_fetch_decode_execute_loop).
+  - intro H_fetch_decode_execute_loop.
+    unfold run.
+    rewrite -> H_fetch_decode_execute_loop.
+    reflexivity.
+  - intros n H_fetch_decode_execute_loop.
+    unfold run.
+    rewrite -> H_fetch_decode_execute_loop.
+    reflexivity.
+  - intros n n' ds'' H_fetch_decode_execute_loop.
+    unfold run.
+    rewrite -> H_fetch_decode_execute_loop.
+    reflexivity.
+ - intros s H_fetch_decode_execute_loop.
+    unfold run.
+    rewrite -> H_fetch_decode_execute_loop.
+    reflexivity.
+Qed.
 
 (* ********** *)
 
